Logic/Modal/Standard/Kripke/Reducible.lean
@@ -10,8 +10,8 @@ namespace Kripke
 open Formula
 
 variable {α : Type*} {Ax₁ Ax₂ : AxiomSet α} (𝔽₁ 𝔽₂ : FrameClass)
-  [sound₁ : Sound Ax₁ᴺ 𝔽₁[α]] [sound₂ : Sound Ax₂ᴺ 𝔽₂[α]]
-  [complete₁ : Complete Ax₁ᴺ 𝔽₁[α]] [complete₂ : Complete Ax₂ᴺ 𝔽₂[α]]
+  [sound₁ : Sound Ax₁ᴺ 𝔽₁#] [sound₂ : Sound Ax₂ᴺ 𝔽₂#]
+  [complete₁ : Complete Ax₁ᴺ 𝔽₁#] [complete₂ : Complete Ax₂ᴺ 𝔽₂#]
 
 lemma reducible_of_subset_FrameClass (h𝔽 : 𝔽₂ ⊆ 𝔽₁) : Ax₁ᴺ ≤ₛ Ax₂ᴺ := by
   apply System.reducible_iff.mpr;
